WIP: working on label logic case

dataplane/Examples/Label_Propagation_op_Correctness.thy
@@ -18,6 +18,8 @@ declare in_filter_zmset_in_zmset[simp del]  pos_filter_zmset_pos_zmset[simp del]
 declare if_cong[cong]
 declare list_emb_Nil2[simp del] BULK_BENQ_right_empty[simp del] BULK_BENQ_left_empty[simp del]
   filter_True[simp del] filter_False[simp del]
+declare cin.rep_eq[simp del]
+declare cin.rep_eq[symmetric, simp]
 
 no_notation shiftr (infixl \<open>>>\<close> 55)
 no_syntax (ASCII) "_thenM" :: \<open>['a, 'b] \<Rightarrow> 'c\<close>  (infixl \<open>>>\<close> 54)
@@ -77,22 +79,22 @@ abbreviation \<open>initial_state_increment inc \<equiv> \<lparr>
 abbreviation \<open>logic_map n \<equiv> map_op (case_option (Inl n) (\<lambda>p. Inr (n, p))) (case_option (Inl n) (\<lambda>p. Inr (n, p)))\<close>
 abbreviation \<open>comp_map \<equiv> map_op (case_sum id id) (case_sum id id)\<close>
 
-abbreviation \<open>op0 state inp \<equiv> Logic (ooo_input_op {|0 :: 2|} (state inp)) default_internal_summary\<close>
+abbreviation \<open>op0 state \<equiv> Logic (ooo_input_op {|0 :: 2|} state) default_internal_summary\<close>
 abbreviation \<open>op1 state \<equiv> Logic (label_propagation_op state) (\<lambda>p1 p2. if p1 = 0 then [0] else if p2 = 1 then [0] else [])\<close>
-abbreviation \<open>op2 state \<equiv> Logic (increment_op (1 :: 2) 1 (MyPair 0 1) (state (MyPair 0 1))) (increment_summary (MyPair 0 1))\<close>
+abbreviation \<open>op2 state \<equiv> Logic (increment_op (1 :: 2) 1 (MyPair 0 1) state) (increment_summary (MyPair 0 1))\<close>
 
-abbreviation G :: "_ \<Rightarrow> _ \<Rightarrow> _ \<Rightarrow> _ \<Rightarrow> (3, 2, (2, (nat, nat) myprod) shared_state + (2 \<Rightarrow> (nat, nat) myprod antichain), (nat \<times> nat + nat set set) \<times> (nat, nat) myprod, (nat, nat) myprod) dataflow_tree" where
-  "G inp_state inp label_state incr_state \<equiv> (Comp [(0, 0) \<mapsto> (0, 0)] (op0 inp_state inp) (Loop [(1, 1) \<mapsto> (0, 1)] (Comp [(0, 1) \<mapsto> (0, 1)] (op1 label_state) (op2 incr_state))))"
+abbreviation G :: "_ \<Rightarrow> _ \<Rightarrow> _ \<Rightarrow> (3, 2, (2, (nat, nat) myprod) shared_state + (2 \<Rightarrow> (nat, nat) myprod antichain), (nat \<times> nat + nat set set) \<times> (nat, nat) myprod, (nat, nat) myprod) dataflow_tree" where
+  "G inp_state label_state incr_state \<equiv> (Comp [(0, 0) \<mapsto> (0, 0)] (op0 inp_state) (Loop [(1, 1) \<mapsto> (0, 1)] (Comp [(0, 1) \<mapsto> (0, 1)] (op1 label_state) (op2 incr_state))))"
 
-abbreviation "compiled inp \<equiv> compile_dataflow (\<lambda> _. []) (G initial_state_input inp initial_state_label_prop initial_state_increment)"
+abbreviation "compiled inp \<equiv> compile_dataflow (\<lambda> _. []) (G (initial_state_input inp) initial_state_label_prop (initial_state_increment (MyPair 0 1)))"
 
-abbreviation "G_op inp_state inp label_state incr_state chns \<equiv>
-   dataflow_tree_to_operator chns (G inp_state inp label_state incr_state)"
+abbreviation "G_op inp_state label_state incr_state chns \<equiv>
+   dataflow_tree_to_operator chns (G inp_state label_state incr_state)"
 
-(* 
+(*
 
 abbreviation \<open>test_input1 \<equiv> llist_of [Mint (MyPair 1 0), Mint (MyPair 2 0), Data \<bottom> (0, 1), Data (MyPair 1 0) (3, 4), Data \<bottom> (1, 2), Data (MyPair 2 0) (4, 5)]\<close>
-value "list_connections (dataflow_tree_to_graph (G initial_state_input test_input1 initial_state_label_prop initial_state_increment))"
+value "list_connections (dataflow_tree_to_graph (G (initial_state_input test_input1) initial_state_label_prop (initial_state_increment (MyPair 0 1))))"
 value [GHC] \<open>ltaken 3 (lmap show_Outs (trace_exec (compiled test_input1)))\<close>
 
 abbreviation \<open>test_input2 \<equiv> llist_of [Mint (MyPair 1 0), Mint (MyPair 2 0), Data \<bottom> (1, 2), Data \<bottom> (0, 1), Data (MyPair 1 0) (3, 4), Data (MyPair 2 0) (4, 5), Mint (MyPair 3 0), Data (MyPair 3 0) (2, 3)]\<close>
@@ -215,7 +217,7 @@ definition \<open>raw_summary = (\<lambda>l1 l2. case (find (\<lambda> (l1', s, 
     Some (l1', s, l2') \<Rightarrow> s :: (nat, nat) myprod list | None \<Rightarrow> [])\<close>
 
 lemma dataflow_tree_to_graph_raw_summary[simp]:
-  "dataflow_tree_to_graph (G inp_state inp label_state incr_state) = raw_summary"
+  "dataflow_tree_to_graph (G inp_state label_state incr_state) = raw_summary"
   unfolding dataflow_tree_to_graph_def Let_def default_internal_summary_def  comp_def                                               
   apply (simp only: split: if_splits prod.splits)
   apply (intro allI impI conjI)
@@ -303,6 +305,11 @@ proof (rule ext)
       (simp_all add: outputs_at_target_def raw_summary_def antichain_from_list_singleton )
 qed
 
+lemma Inr_2_1_in_ran[simp]:
+  "Inr (2 :: 3, 1 :: 2) \<in> ran (case_sum (\<lambda>_. None) (\<lambda>(nid, p). case if nid = 1 \<and> p = 1 then Some (0, 1) else None of None \<Rightarrow> None | Some (offset, q) \<Rightarrow> Some (Inr (1 + 1 + offset, q))))"
+  unfolding ran_def
+  by (auto split: sum.splits if_splits)
+
 lemma label_propagation_correctness:
   fixes lxs :: \<open>((nat, nat) myprod, nat \<times> nat) event llist\<close>
     and os :: \<open>3 \<Rightarrow> (2, nat \<times> nat + nat set set, (nat, nat) myprod) operator_state\<close>
@@ -315,9 +322,6 @@ lemma label_propagation_correctness:
     and V :: \<open>nat \<Rightarrow> nat list\<close>
     and L :: \<open>nat \<Rightarrow> nat \<Rightarrow> nat\<close>
     and S SO SP D :: \<open>((3 \<times> 2) \<times> (nat \<times> nat + nat set set) \<times> (nat, nat) myprod) cset\<close>
-  defines \<open>my_ooo_input_op os' \<equiv> logic_map (0 :: 3) (ooo_input_op {|0 :: 2|} os')\<close>
-    and \<open>my_label_propagation_op os'' \<equiv> logic_map (1 :: 3) (label_propagation_op os'')\<close>
-    and \<open>my_increment_op os''' \<equiv> logic_map (2 :: 3) (increment_op (0 :: 2) 0 (MyPair (0 :: nat) (Suc 0)) os''')\<close>
   assumes
     subgraph_inv: \<open>summ sg = antichain_from_list \<circ>\<circ> raw_summary\<close> \<open>nxt sg = graph_to_nxt (summ sg)\<close>
     and
@@ -339,15 +343,9 @@ lemma label_propagation_correctness:
       (cUn (ts lxs) (cset_from_list (map snd (chns (1, 0)))))\<close>
     \<open>SO = cset_from_list (map (\<lambda>x. ((1, 0), x)) (outpu (os 1) 0))\<close>
     and input_stream_inv: \<open>timely_input_stream lxs (mset (ocaps (os 0) 0))\<close>
-  shows \<open>set_op S D (dataflow_op sg
-  (comp_map (comp_op [Inr (0, 0) \<mapsto> Inr (1, 0)] (\<lambda>x. case x of Inl _ \<Rightarrow> [] | Inr l \<Rightarrow> map Inr (cbufs l))
-    (my_ooo_input_op os_input)
-    (loop_op [Inr (2, 0) \<mapsto> Inr (1, 1)] (\<lambda>x. case x of Inl _ \<Rightarrow> [] | Inr l \<Rightarrow> map Inr (cbufs l))
-      (comp_map (comp_op [Inr (1, 1) \<mapsto> Inr (2, 0)] (\<lambda>x. case x of Inl _ \<Rightarrow> [] | Inr l \<Rightarrow> map Inr (cbufs l))
-        (my_label_propagation_op os_label_prop)
-        (my_increment_op (os 2))))))))
-  \<approx> set_spec_op (cUn (cUn S SO) SP) D\<close>
-  using assms(4-)
+  shows \<open>set_op S D (dataflow_op sg (G_op os_input os_label_prop (os 2) chns))
+         \<approx> set_spec_op (cUn (cUn S SO) SP) D\<close>
+  using assms
 proof (coinduction arbitrary: S SO SP D lxs os os_input os_label_prop cbufs chns sg T G V L
     rule: weakBisimWeakUptoBisimCong)
   case SIM1
@@ -358,155 +356,263 @@ proof (coinduction arbitrary: S SO SP D lxs os os_input os_label_prop cbufs chns
     show ?thesis
       using [[goals_limit=16]]
       unfolding R_def[symmetric]
-      unfolding wsim_def my_ooo_input_op_def ooo_input_op_def my_label_propagation_op_def label_propagation_op_def my_increment_op_def increment_op_def
+      unfolding wsim_def dataflow_tree_to_operator_def  ooo_input_op_def label_propagation_op_def increment_op_def
+      apply simp
       apply (intro allI impI)
       apply ((elim step_dataflow_op_elim step_set_op_elim step_map_op_elim step_comp_op_elim
-          step_builder_op_elim conjE; simp only: IO.simps; hypsubst_thin?; (elim step_map_op_elim
-            step_comp_op_elim step_loop_op_elim step_builder_op_elim conjE)?), simp_all only: IO.simps;
-        clarsimp split: if_splits option.splits dest!: num2_neq simp flip: my_ooo_input_op_def ooo_input_op_def my_label_propagation_op_def label_propagation_op_def my_increment_op_def increment_op_def; hypsubst_thin?)
+            step_builder_op_elim conjE; simp only: IO.simps; hypsubst_thin?; (elim step_map_op_elim
+              step_comp_op_elim step_loop_op_elim step_builder_op_elim conjE)?), simp_all only: IO.simps;
+          clarsimp split: if_splits option.splits dest!: num2_neq simp flip:  ooo_input_op_def label_propagation_op_def increment_op_def; hypsubst_thin?)
+                     prefer 7
+      subgoal for os'
+        unfolding label_propagation_op_logic_def trace_simp
+        apply clarsimp
+        apply (elim disjE)
+          prefer 3
+        subgoal
+          apply (simp split: if_splits prod.splits)
+          apply hypsubst_thin
+          apply (intro exI conjI relcomppI)
+             apply (rule rtranclp.intros(1))
+            apply (rule bisim_refl)
+           defer
+           apply (rule wbisim_refl)
+          apply (rule wb_upto_b_base)
+          unfolding R_def[simplified]
+          apply (rule exI[of _ S])
+          apply (rule exI[of _ D])
+          apply (rule exI[of _ lxs])
+          apply (rule exI[of _ "os(1 := drop_caps
+                       (produces (release_caps (os 1) 1)
+                         (map (\<lambda>t. (en2 os_label_prop
+                                      (all_vertices (release_caps os_label_prop 1) t //
+                                       {(v1, v2).
+                                        v1 \<in> all_vertices (release_caps os_label_prop 1) t \<and>
+                                        v2 \<in> all_vertices (release_caps os_label_prop 1) t \<and> min_label (release_caps os_label_prop 1) t v1 = min_label (release_caps os_label_prop 1) t v2}),
+                                     Cap (MyPair t 0) 0))
+                           (mergesort_remdups
+                             (map myfst
+                               (filter (\<lambda>t. \<not> frontier_less_equal (exit_scope myfst (front (release_caps (os 1) 1) 0 + front (release_caps (os 1) 1) 1)) (myfst t))
+                                 (ocaps (release_caps (os 1) 1) 0))))))
+                       (map (\<lambda>t. Cap t 0)
+                         (filter (\<lambda>t. \<not> frontier_less_equal (exit_scope myfst (front (release_caps (os 1) 1) 0 + front (release_caps (os 1) 1) 1)) (myfst t))
+                           (ocaps (release_caps os_label_prop 1) 0)) @
+                        map (\<lambda>t. Cap t 1)
+                         (filter (\<lambda>t. \<not> frontier_less_equal (exit_scope myfst (front (release_caps (os 1) 1) 0 + front (release_caps (os 1) 1) 1)) (myfst t))
+                           (ocaps (release_caps (os 1) 1) 1))))"])
+          apply (rule exI[of _ "drop_caps
+                       (produces (release_caps os_label_prop 1)
+                         (map (\<lambda>t. (en2 (release_caps os_label_prop 1)
+                                      (all_vertices (release_caps os_label_prop 1) t //
+                                       {(v1, v2).
+                                        v1 \<in> all_vertices (release_caps os_label_prop 1) t \<and>
+                                        v2 \<in> all_vertices (release_caps os_label_prop 1) t \<and> min_label (release_caps os_label_prop 1) t v1 = min_label (release_caps os_label_prop 1) t v2}),
+                                     Cap (MyPair t 0) 0))
+                           (mergesort_remdups
+                             (map myfst
+                               (filter (\<lambda>t. \<not> frontier_less_equal (exit_scope myfst (front (release_caps os_label_prop 1) 0 + front (release_caps os_label_prop 1) 1)) (myfst t))
+                                 (ocaps (release_caps os_label_prop 1) 0))))))
+                       (map (\<lambda>t. Cap t 0)
+                         (filter (\<lambda>t. \<not> frontier_less_equal (exit_scope myfst (front (release_caps os_label_prop 1) 0 + front (release_caps os_label_prop 1) 1)) (myfst t))
+                           (ocaps (release_caps os_label_prop 1) 0)) @
+                        map (\<lambda>t. Cap t 1)
+                         (filter (\<lambda>t. \<not> frontier_less_equal (exit_scope myfst (front (release_caps os_label_prop 1) 0 + front (release_caps os_label_prop 1) 1)) (myfst t))
+                           (ocaps (release_caps os_label_prop 1) 1)))"])
+          apply (rule exI[of _ cbufs])
+          apply (rule exI[of _ sg])
+          apply (intro conjI)
+          subgoal
+            apply simp
+            apply (simp add: dataflow_tree_to_operator_def SIM1(3))
+            apply (rule arg_cong3[where f=set_op])
+              apply simp
+             apply simp
+            apply (rule arg_cong2[where f=dataflow_op])
+             apply simp
+            apply (rule arg_cong[where f=comp_map])
+            apply (rule arg_cong4[where f=comp_op])
+               apply simp
+              apply (simp add: SIM1(11))
+            subgoal premises aux
+              apply (rule ext)+
+              unfolding BULK_BENQ_def
+              apply (simp add: operator_state.defs)
+              apply (rule arg_cong2[where f=append])
+              subgoal
+                apply (rule map_cong)
+                 apply simp_all
+                unfolding drop_caps_def produces_def release_caps_def inputs_at_target_def
+                apply (simp split: prod.splits)
+                done
+              subgoal
+                apply (rule arg_cong2[where f=append])
+                subgoal
+                  by simp
+                subgoal
+                  apply (rule map_cong)
+                   apply (simp_all add: SIM1(1) outputs_at_target_raw_summary release_caps_def filter_empty_conv)
+                  done
+                done
+              done
+            subgoal by simp
+            subgoal
+              apply (rule arg_cong3[where f=loop_op])
+                apply simp
+              subgoal premises aux
+                by (auto cong: map_cong simp add: BULK_BENQ_def SIM1(11) drop_caps_def produces_def inputs_at_target_def operator_state.defs SIM1(1) outputs_at_target_raw_summary release_caps_def filter_empty_conv split: sum.splits)
+              apply (rule arg_cong[where f=comp_map])
+              apply (rule arg_cong4[where f=comp_op])
+                 apply simp
+              subgoal premises aux
+                by (auto cong: map_cong simp add: BULK_BENQ_def SIM1(11) drop_caps_def produces_def inputs_at_target_def operator_state.defs SIM1(1) outputs_at_target_raw_summary release_caps_def filter_empty_conv split: sum.splits)
+               apply simp
+              apply simp
+              done
+            done
 
 
+          find_theorems chns
 
 end
-    have "\<exists>op2'. step (Out (n, p) (d, t)) (set_spec_op (cUn (cUn S SO) SP) D) op2' \<and> ((~) OO \<U> R OO (\<approx>)) (set_op S (cinsert ((n, p), d, t) D) (dataflow_op sg (comp_map (comp_op [Inr (0, 0) \<mapsto> Inr (1, 0)] (case_sum (\<lambda>x. []) (\<lambda>l. map Inr (cbufs l))) (my_ooo_input_op os_input) (loop_op [Inr (2, 0) \<mapsto> Inr (1, 1)] (case_sum (\<lambda>x. []) (\<lambda>l. map Inr (cbufs l))) (comp_map (comp_op [Inr (1, 1) \<mapsto> Inr (2, 0)] (case_sum (\<lambda>x. []) (\<lambda>l. map Inr (cbufs l))) (my_label_propagation_op os_label_prop) (my_increment_op (os 2))))))))) op2'"
-      (is \<open>\<exists>_. step _ ?op2 _ \<and> ((~) OO \<U> R OO (\<approx>)) ?op1' _\<close>)
-      if "((n, p), d, t) |\<in>| S"
-        and "\<not> ((n, p), d, t) |\<in>| D"
-      for n :: "3"
-        and p :: "2"
-        and d :: "nat \<times> nat + nat set set"
-        and t :: "(nat, nat) myprod"
-    proof -
-      have \<open>R ?op1' (set_spec_op (cUn (cUn S SO) SP) (cinsert ((n, p), d, t) D))\<close> unfolding R_def
-        by (intro exI conjI) (use SIM1 in \<open>simp_all add: comp_def\<close>)
-      thus ?thesis using bisim_refl wbisim_refl wb_upto_b_base step_set_spec_op_intro_Out that by blast
-    qed
-    moreover have "\<exists>op2'. (step Tau)\<^sup>*\<^sup>* (set_spec_op (cUn (cUn S SO) SP) D) op2' \<and> ((~) OO \<U> R OO (\<approx>)) (set_op S D (dataflow_op sg (comp_map (comp_op [Inr (0, 0) \<mapsto> Inr (1, 0)] (case_sum (\<lambda>x. []) (BENQ (1, 0) (Inr (d, t)) (\<lambda>l. map Inr (cbufs l)))) (my_ooo_input_op (os_input\<lparr>outpu := (outpu os_input)(0 := xs)\<rparr>)) (loop_op [Inr (2, 0) \<mapsto> Inr (1, 1)] (case_sum (\<lambda>x. []) (\<lambda>l. map Inr (cbufs l))) (comp_map (comp_op [Inr (1, 1) \<mapsto> Inr (2, 0)] (case_sum (\<lambda>x. []) (\<lambda>l. map Inr (cbufs l))) (my_label_propagation_op os_label_prop) (my_increment_op (os 2))))))))) op2'"
-      if "outpu os_input 0 = (d, t) # xs"
-      for d :: "nat \<times> nat + nat set set"
-        and t :: "(nat, nat) myprod"
-        and xs :: "((nat \<times> nat + nat set set) \<times> (nat, nat) myprod) buf"
-      using that sorry
-    moreover have "\<exists>op2'. (step Tau)\<^sup>*\<^sup>* (set_spec_op (cUn (cUn S SO) SP) D) op2' \<and> ((~) OO \<U> R OO (\<approx>)) (set_op S D (dataflow_op sg (comp_map (comp_op [Inr (0, 0) \<mapsto> Inr (1, 0)] (case_sum (\<lambda>x. []) (BTL (1, 0) (\<lambda>l. map Inr (cbufs l)))) (my_ooo_input_op os_input) (loop_op [Inr (2, 0) \<mapsto> Inr (1, 1)] (case_sum (\<lambda>x. []) (\<lambda>l. map Inr (cbufs l))) (comp_map (comp_op [Inr (1, 1) \<mapsto> Inr (2, 0)] (case_sum (\<lambda>x. []) (\<lambda>l. map Inr (cbufs l))) (my_label_propagation_op (consumes os_label_prop 0 t d)) (my_increment_op (os 2))))))))) op2'"
-      if "cbufs (1, 0) \<noteq> []"
-        and "(d, t) = BHD (1, 0) cbufs"
-      for d :: "nat \<times> nat + nat set set"
-        and t :: "(nat, nat) myprod"
-      using that sorry
-    moreover have "\<exists>op2'. (step Tau)\<^sup>*\<^sup>* (set_spec_op (cUn (cUn S SO) SP) D) op2' \<and> ((~) OO \<U> R OO (\<approx>)) (set_op S D (dataflow_op sg (comp_map (comp_op [Inr (0, 0) \<mapsto> Inr (1, 0)] (case_sum (\<lambda>x. []) (\<lambda>l. map Inr (cbufs l))) (my_ooo_input_op os') (loop_op [Inr (2, 0) \<mapsto> Inr (1, 1)] (case_sum (\<lambda>x. []) (\<lambda>l. map Inr (cbufs l))) (comp_map (comp_op [Inr (1, 1) \<mapsto> Inr (2, 0)] (case_sum (\<lambda>x. []) (\<lambda>l. map Inr (cbufs l))) (my_label_propagation_op os_label_prop) (my_increment_op (os 2))))))))) op2'"
-      if "initia os_input"
-        and "os' |\<in>| ooo_input_op_logic {|0|} os_input"
-      for os' :: "(2, nat \<times> nat + nat set set, nat \<times> nat, (nat, nat) myprod) input_state"
-      using that sorry
-    moreover have "\<exists>op2'. (step Tau)\<^sup>*\<^sup>* (set_spec_op (cUn (cUn S SO) SP) D) op2' \<and> ((~) OO \<U> R OO (\<approx>)) (set_op S D (dataflow_op sg (comp_map (comp_op [Inr (0, 0) \<mapsto> Inr (1, 0)] (case_sum (\<lambda>x. []) (\<lambda>l. map Inr (cbufs l))) (my_ooo_input_op os_input) (loop_op [Inr (2, 0) \<mapsto> Inr (1, 1)] (case_sum (\<lambda>x. []) (\<lambda>l. map Inr (cbufs l))) (comp_map (comp_op [Inr (1, 1) \<mapsto> Inr (2, 0)] (case_sum (\<lambda>x. []) (BENQ (2, 0) (Inr (d, t)) (\<lambda>l. map Inr (cbufs l)))) (my_label_propagation_op (os_label_prop \<lparr>outpu := (outpu os_label_prop)(1 := xs)\<rparr>)) (my_increment_op (os 2))))))))) op2'"
-      if "outpu os_label_prop 1 = (d, t) # xs"
-      for d :: "nat \<times> nat + nat set set"
-        and t :: "(nat, nat) myprod"
-        and xs :: "((nat \<times> nat + nat set set) \<times> (nat, nat) myprod) buf"
-      using that sorry
-    moreover have "\<exists>op2'. (step Tau)\<^sup>*\<^sup>* (set_spec_op (cUn (cUn S SO) SP) D) op2' \<and> ((~) OO \<U> R OO (\<approx>)) (set_op S D (dataflow_op sg (comp_map (comp_op [Inr (0, 0) \<mapsto> Inr (1, 0)] (case_sum (\<lambda>x. []) (\<lambda>l. map Inr (cbufs l))) (my_ooo_input_op os_input) (loop_op [Inr (2, 0) \<mapsto> Inr (1, 1)] (case_sum (\<lambda>x. []) (\<lambda>l. map Inr (cbufs l))) (comp_map (comp_op [Inr (1, 1) \<mapsto> Inr (2, 0)] (case_sum (\<lambda>x. []) (BTL (2, 0) (\<lambda>l. map Inr (cbufs l)))) (my_label_propagation_op os_label_prop) (my_increment_op (consumes (os 2) 0 t d))))))))) op2'"
-      if "cbufs (2, 0) \<noteq> []"
-        and "(d, t) = BHD (2, 0) cbufs"
-      for d :: "nat \<times> nat + nat set set"
-        and t :: "(nat, nat) myprod"
-      using that sorry
-    moreover have "\<exists>op2'. (step Tau)\<^sup>*\<^sup>* (set_spec_op (cUn (cUn S SO) SP) D) op2' \<and> ((~) OO \<U> R OO (\<approx>)) (set_op S D (dataflow_op sg (comp_map (comp_op [Inr (0, 0) \<mapsto> Inr (1, 0)] (case_sum (\<lambda>x. []) (\<lambda>l. map Inr (cbufs l))) (my_ooo_input_op os_input) (loop_op [Inr (2, 0) \<mapsto> Inr (1, 1)] (case_sum (\<lambda>x. []) (\<lambda>l. map Inr (cbufs l))) (comp_map (comp_op [Inr (1, 1) \<mapsto> Inr (2, 0)] (case_sum (\<lambda>x. []) (\<lambda>l. map Inr (cbufs l))) (my_label_propagation_op os') (my_increment_op (os 2))))))))) op2'"
-      if "initia os_label_prop"
-        and "os' |\<in>| label_propagation_op_logic os_label_prop"
-      for os' :: "(nat \<times> nat + nat set set, nat, nat, nat) label_propagation_state"
-      using that sorry
-    moreover have "\<exists>op2'. (step Tau)\<^sup>*\<^sup>* (set_spec_op (cUn (cUn S SO) SP) D) op2' \<and> ((~) OO \<U> R OO (\<approx>)) (set_op S D (dataflow_op sg (comp_map (comp_op [Inr (0, 0) \<mapsto> Inr (1, 0)] (case_sum (\<lambda>x. []) (\<lambda>l. map Inr (cbufs l))) (my_ooo_input_op os_input) (loop_op [Inr (2, 0) \<mapsto> Inr (1, 1)] (case_sum (\<lambda>x. []) (\<lambda>l. map Inr (cbufs l))) (comp_map (comp_op [Inr (1, 1) \<mapsto> Inr (2, 0)] (case_sum (\<lambda>x. []) (\<lambda>l. map Inr (cbufs l))) (my_label_propagation_op os_label_prop) (my_increment_op os')))))))) op2'"
-      if "initia (os 2)"
-        and "os' |\<in>| increment_op_logic 0 0 (MyPair 0 1) (os 2)"
-      for os' :: "(2, nat \<times> nat + nat set set, (nat, nat) myprod) operator_state"
-      using that sorry
-    moreover have "\<exists>op2'. (step Tau)\<^sup>*\<^sup>* (set_spec_op (cUn (cUn S SO) SP) D) op2' \<and> ((~) OO \<U> R OO (\<approx>)) (set_op S D (dataflow_op sg (comp_map (comp_op [Inr (0, 0) \<mapsto> Inr (1, 0)] (case_sum (\<lambda>x. []) (\<lambda>l. map Inr (cbufs l))) (my_ooo_input_op os_input) (loop_op [Inr (2, 0) \<mapsto> Inr (1, 1)] (case_sum (\<lambda>x. []) (BTL (1, 1) (\<lambda>l. map Inr (cbufs l)))) (comp_map (comp_op [Inr (1, 1) \<mapsto> Inr (2, 0)] (case_sum (\<lambda>x. []) (\<lambda>l. map Inr (cbufs l))) (my_label_propagation_op (consumes os_label_prop 1 t d)) (my_increment_op (os 2))))))))) op2'"
-      if "cbufs (1, 1) \<noteq> []"
-        and "(d, t) = BHD (1, 1) cbufs"
-      for d :: "nat \<times> nat + nat set set"
-        and t :: "(nat, nat) myprod"
-      using that sorry
-    moreover have "\<exists>op2'. (step Tau)\<^sup>*\<^sup>* (set_spec_op (cUn (cUn S SO) SP) D) op2' \<and> ((~) OO \<U> R OO (\<approx>)) (set_op S D (dataflow_op sg (comp_map (comp_op [Inr (0, 0) \<mapsto> Inr (1, 0)] (case_sum (\<lambda>x. []) (\<lambda>l. map Inr (cbufs l))) (my_ooo_input_op os_input) (loop_op [Inr (2, 0) \<mapsto> Inr (1, 1)] (case_sum (\<lambda>x. []) (BENQ (1, 1) (Inr (d, t)) (\<lambda>l. map Inr (cbufs l)))) (comp_map (comp_op [Inr (1, 1) \<mapsto> Inr (2, 0)] (case_sum (\<lambda>x. []) (\<lambda>l. map Inr (cbufs l))) (my_label_propagation_op os_label_prop) (my_increment_op (os 2\<lparr>outpu := (outpu (os 2))(0 := xs)\<rparr>))))))))) op2'"
-      if "outpu (os 2) 0 = (d, t) # xs"
-      for d :: "nat \<times> nat + nat set set"
-        and t :: "(nat, nat) myprod"
-        and xs :: "((nat \<times> nat + nat set set) \<times> (nat, nat) myprod) buf"
-      using that sorry
-    moreover have "\<exists>op2'. (step Tau)\<^sup>*\<^sup>* (set_spec_op (cUn (cUn S SO) SP) D) op2' \<and> ((~) OO \<U> R OO (\<approx>)) (set_op S D (dataflow_op (sg\<lparr>upfro := \<lambda>_. True, pt_tr := change_multiplicities (summ sg) (extract_progress 2 (subgraph.nxt sg) st) (pt_tr sg)\<rparr>) (comp_map (comp_op [Inr (0, 0) \<mapsto> Inr (1, 0)] (case_sum (\<lambda>x. []) (\<lambda>l. map Inr (cbufs l))) (my_ooo_input_op os_input) (loop_op [Inr (2, 0) \<mapsto> Inr (1, 1)] (case_sum (\<lambda>x. []) (\<lambda>l. map Inr (cbufs l))) (comp_map (comp_op [Inr (1, 1) \<mapsto> Inr (2, 0)] (case_sum (\<lambda>x. []) (\<lambda>l. map Inr (cbufs l))) (my_label_propagation_op os_label_prop) (my_increment_op os')))))))) op2'"
-      if "(os', st) = obtain_progress (os 2)"
-      for st :: "(2, (nat, nat) myprod) shared_state"
-        and os' :: "(2, nat \<times> nat + nat set set, (nat, nat) myprod) operator_state"
-      using that sorry
-    moreover have "\<exists>op2'. (step Tau)\<^sup>*\<^sup>* (set_spec_op (cUn (cUn S SO) SP) D) op2' \<and> ((~) OO \<U> R OO (\<approx>)) (set_op S D (dataflow_op (sg\<lparr>upfro := \<lambda>_. True, pt_tr := change_multiplicities (summ sg) (extract_progress 1 (subgraph.nxt sg) st) (pt_tr sg)\<rparr>) (comp_map (comp_op [Inr (0, 0) \<mapsto> Inr (1, 0)] (case_sum (\<lambda>x. []) (\<lambda>l. map Inr (cbufs l))) (my_ooo_input_op os_input) (loop_op [Inr (2, 0) \<mapsto> Inr (1, 1)] (case_sum (\<lambda>x. []) (\<lambda>l. map Inr (cbufs l))) (comp_map (comp_op [Inr (1, 1) \<mapsto> Inr (2, 0)] (case_sum (\<lambda>x. []) (\<lambda>l. map Inr (cbufs l))) (my_label_propagation_op os') (my_increment_op (os 2))))))))) op2'"
-      if "(os', st) = obtain_progress os_label_prop"
-      for st :: "(2, (nat, nat) myprod) shared_state"
-        and os' :: "(nat \<times> nat + nat set set, nat, nat, nat) label_propagation_state"
-      using that sorry
-    moreover have "\<exists>op2'. (step Tau)\<^sup>*\<^sup>* (set_spec_op (cUn (cUn S SO) SP) D) op2' \<and> ((~) OO \<U> R OO (\<approx>)) (set_op S D (dataflow_op (sg\<lparr>upfro := \<lambda>_. True, pt_tr := change_multiplicities (summ sg) (extract_progress 0 (subgraph.nxt sg) st) (pt_tr sg)\<rparr>) (comp_map (comp_op [Inr (0, 0) \<mapsto> Inr (1, 0)] (case_sum (\<lambda>x. []) (\<lambda>l. map Inr (cbufs l))) (my_ooo_input_op os') (loop_op [Inr (2, 0) \<mapsto> Inr (1, 1)] (case_sum (\<lambda>x. []) (\<lambda>l. map Inr (cbufs l))) (comp_map (comp_op [Inr (1, 1) \<mapsto> Inr (2, 0)] (case_sum (\<lambda>x. []) (\<lambda>l. map Inr (cbufs l))) (my_label_propagation_op os_label_prop) (my_increment_op (os 2))))))))) op2'"
-      if "(os', st) = obtain_progress os_input"
-      for st :: "(2, (nat, nat) myprod) shared_state"
-        and os' :: "(2, nat \<times> nat + nat set set, nat \<times> nat, (nat, nat) myprod) input_state"
-      using that sorry
-    moreover have "\<exists>op2'. (step Tau)\<^sup>*\<^sup>* (set_spec_op (cUn (cUn S SO) SP) D) op2' \<and> ((~) OO \<U> R OO (\<approx>)) (set_op S D (dataflow_op undefined (comp_map (comp_op [Inr (0, 0) \<mapsto> Inr (1, 0)] (case_sum (\<lambda>x. []) (\<lambda>l. map Inr (cbufs l))) (my_ooo_input_op os_input) (loop_op [Inr (2, 0) \<mapsto> Inr (1, 1)] (case_sum (\<lambda>x. []) (\<lambda>l. map Inr (cbufs l))) (comp_map (comp_op [Inr (1, 1) \<mapsto> Inr (2, 0)] (case_sum (\<lambda>x. []) (\<lambda>l. map Inr (cbufs l))) (my_label_propagation_op (os_label_prop \<lparr>front := frontier \<circ> (\<lambda>p. c_imp (pt_tr undefined) (Loc 1 (Trg p))), initia := True\<rparr>)) (my_increment_op (os 2))))))))) op2'"
-      if "propagate_all (summ sg) (pt_tr sg) = None"
-      using that sorry
-    moreover have "\<exists>op2'. (step Tau)\<^sup>*\<^sup>* (set_spec_op (cUn (cUn S SO) SP) D) op2' \<and> ((~) OO \<U> R OO (\<approx>)) (set_op S D (dataflow_op (sg\<lparr>pt_tr := c, upfro := (upfro sg)(1 := False)\<rparr>) (comp_map (comp_op [Inr (0, 0) \<mapsto> Inr (1, 0)] (case_sum (\<lambda>x. []) (\<lambda>l. map Inr (cbufs l))) (my_ooo_input_op os_input) (loop_op [Inr (2, 0) \<mapsto> Inr (1, 1)] (case_sum (\<lambda>x. []) (\<lambda>l. map Inr (cbufs l))) (comp_map (comp_op [Inr (1, 1) \<mapsto> Inr (2, 0)] (case_sum (\<lambda>x. []) (\<lambda>l. map Inr (cbufs l))) (my_label_propagation_op (os_label_prop \<lparr>front := frontier \<circ> (\<lambda>p. c_imp c (Loc 1 (Trg p))), initia := True\<rparr>)) (my_increment_op (os 2))))))))) op2'"
-      if "propagate_all (summ sg) (pt_tr sg) = Some c"
-      for c :: "((3, 2) location, (nat, nat) myprod) configuration"
-      using that sorry
-    moreover have "\<exists>op2'. (step Tau)\<^sup>*\<^sup>* (set_spec_op (cUn (cUn S SO) SP) D) op2' \<and> ((~) OO \<U> R OO (\<approx>)) (set_op (cinsert ((1, 0), d, t) S) D (dataflow_op sg (comp_map (comp_op [Inr (0, 0) \<mapsto> Inr (1, 0)] (case_sum (\<lambda>x. []) (\<lambda>l. map Inr (cbufs l))) (my_ooo_input_op os_input) (loop_op [Inr (2, 0) \<mapsto> Inr (1, 1)] (case_sum (\<lambda>x. []) (\<lambda>l. map Inr (cbufs l))) (comp_map (comp_op [Inr (1, 1) \<mapsto> Inr (2, 0)] (case_sum (\<lambda>x. []) (\<lambda>l. map Inr (cbufs l))) (my_label_propagation_op (os_label_prop \<lparr>outpu := (outpu os_label_prop)(0 := xs)\<rparr>)) (my_increment_op (os 2))))))))) op2'"
-      if "outpu os_label_prop 0 = (d, t) # xs"
-      for d :: "nat \<times> nat + nat set set"
-        and t :: "(nat, nat) myprod"
-        and xs :: "((nat \<times> nat + nat set set) \<times> (nat, nat) myprod) buf"
-      apply (intro exI conjI)
-       apply (rule rtranclp.rtrancl_refl)
-      apply (intro relcomppI)
-        apply (rule bisim_refl)
-       defer
-       apply (rule wbisim_refl)
-      apply (rule wb_upto_b_base)
-      apply (unfold R_def)
-      apply (rule exI[of _ \<open>cinsert ((1, 0), d, t) S\<close>])
-      apply (rule exI[of _ \<open>cset_from_list (map (\<lambda>x. ((1, 0), x)) xs)\<close>])
-      apply (rule exI[of _ SP])
-      apply (rule exI)
-      apply (rule exI)
-      apply (rule exI[of _ \<open>os(1 := (os 1)\<lparr>outpu := (outpu (os 1))(0 := xs)\<rparr>)\<close>])
-      apply (rule exI)
-      apply (rule exI[of _ \<open>os_label_prop\<lparr>outpu := (outpu os_label_prop)(0 := xs)\<rparr>\<close>])
-      apply (intro exI conjI)
-                      apply simp
-                     apply (rule arg_cong[where f=\<open>\<lambda>X. set_spec_op (cUn X SP) D\<close>])
-      using SIM1(6,14) that apply (simp add: operator_state.defs(3))
-                    apply (simp_all add: SIM1 operator_state.defs(3))
-      using SIM1(3,7) unfolding ty1_check_def apply (simp add: operator_state.defs(3), blast)
-      subgoal
-        using SIM1(6,8) that unfolding ty2_check_def apply -
-        by (simp add: operator_state.defs(3), drule spec[of _ 0], simp)
-      using SIM1(9) unfolding input_ocaps_inv_def apply simp
-        defer
-        apply (subgoal_tac \<open>outputs_at_target (antichain_from_list \<circ>\<circ> raw_summary) (os(1 := (os 1)\<lparr>outpu := (outpu (os 1))(0 := xs)\<rparr>)) (1, 0)
+  have "\<exists>op2'. step (Out (n, p) (d, t)) (set_spec_op (cUn (cUn S SO) SP) D) op2' \<and> ((~) OO \<U> R OO (\<approx>)) (set_op S (cinsert ((n, p), d, t) D) (dataflow_op sg (comp_map (comp_op [Inr (0, 0) \<mapsto> Inr (1, 0)] (case_sum (\<lambda>x. []) (\<lambda>l. map Inr (cbufs l))) (my_ooo_input_op os_input) (loop_op [Inr (2, 0) \<mapsto> Inr (1, 1)] (case_sum (\<lambda>x. []) (\<lambda>l. map Inr (cbufs l))) (comp_map (comp_op [Inr (1, 1) \<mapsto> Inr (2, 0)] (case_sum (\<lambda>x. []) (\<lambda>l. map Inr (cbufs l))) (my_label_propagation_op os_label_prop) (my_increment_op (os 2))))))))) op2'"
+    (is \<open>\<exists>_. step _ ?op2 _ \<and> ((~) OO \<U> R OO (\<approx>)) ?op1' _\<close>)
+    if "((n, p), d, t) |\<in>| S"
+      and "\<not> ((n, p), d, t) |\<in>| D"
+    for n :: "3"
+      and p :: "2"
+      and d :: "nat \<times> nat + nat set set"
+      and t :: "(nat, nat) myprod"
+  proof -
+    have \<open>R ?op1' (set_spec_op (cUn (cUn S SO) SP) (cinsert ((n, p), d, t) D))\<close> unfolding R_def
+      by (intro exI conjI) (use SIM1 in \<open>simp_all add: comp_def\<close>)
+    thus ?thesis using bisim_refl wbisim_refl wb_upto_b_base step_set_spec_op_intro_Out that by blast
+  qed
+  moreover have "\<exists>op2'. (step Tau)\<^sup>*\<^sup>* (set_spec_op (cUn (cUn S SO) SP) D) op2' \<and> ((~) OO \<U> R OO (\<approx>)) (set_op S D (dataflow_op sg (comp_map (comp_op [Inr (0, 0) \<mapsto> Inr (1, 0)] (case_sum (\<lambda>x. []) (BENQ (1, 0) (Inr (d, t)) (\<lambda>l. map Inr (cbufs l)))) (my_ooo_input_op (os_input\<lparr>outpu := (outpu os_input)(0 := xs)\<rparr>)) (loop_op [Inr (2, 0) \<mapsto> Inr (1, 1)] (case_sum (\<lambda>x. []) (\<lambda>l. map Inr (cbufs l))) (comp_map (comp_op [Inr (1, 1) \<mapsto> Inr (2, 0)] (case_sum (\<lambda>x. []) (\<lambda>l. map Inr (cbufs l))) (my_label_propagation_op os_label_prop) (my_increment_op (os 2))))))))) op2'"
+    if "outpu os_input 0 = (d, t) # xs"
+    for d :: "nat \<times> nat + nat set set"
+      and t :: "(nat, nat) myprod"
+      and xs :: "((nat \<times> nat + nat set set) \<times> (nat, nat) myprod) buf"
+    using that sorry
+  moreover have "\<exists>op2'. (step Tau)\<^sup>*\<^sup>* (set_spec_op (cUn (cUn S SO) SP) D) op2' \<and> ((~) OO \<U> R OO (\<approx>)) (set_op S D (dataflow_op sg (comp_map (comp_op [Inr (0, 0) \<mapsto> Inr (1, 0)] (case_sum (\<lambda>x. []) (BTL (1, 0) (\<lambda>l. map Inr (cbufs l)))) (my_ooo_input_op os_input) (loop_op [Inr (2, 0) \<mapsto> Inr (1, 1)] (case_sum (\<lambda>x. []) (\<lambda>l. map Inr (cbufs l))) (comp_map (comp_op [Inr (1, 1) \<mapsto> Inr (2, 0)] (case_sum (\<lambda>x. []) (\<lambda>l. map Inr (cbufs l))) (my_label_propagation_op (consumes os_label_prop 0 t d)) (my_increment_op (os 2))))))))) op2'"
+    if "cbufs (1, 0) \<noteq> []"
+      and "(d, t) = BHD (1, 0) cbufs"
+    for d :: "nat \<times> nat + nat set set"
+      and t :: "(nat, nat) myprod"
+    using that sorry
+  moreover have "\<exists>op2'. (step Tau)\<^sup>*\<^sup>* (set_spec_op (cUn (cUn S SO) SP) D) op2' \<and> ((~) OO \<U> R OO (\<approx>)) (set_op S D (dataflow_op sg (comp_map (comp_op [Inr (0, 0) \<mapsto> Inr (1, 0)] (case_sum (\<lambda>x. []) (\<lambda>l. map Inr (cbufs l))) (my_ooo_input_op os') (loop_op [Inr (2, 0) \<mapsto> Inr (1, 1)] (case_sum (\<lambda>x. []) (\<lambda>l. map Inr (cbufs l))) (comp_map (comp_op [Inr (1, 1) \<mapsto> Inr (2, 0)] (case_sum (\<lambda>x. []) (\<lambda>l. map Inr (cbufs l))) (my_label_propagation_op os_label_prop) (my_increment_op (os 2))))))))) op2'"
+    if "initia os_input"
+      and "os' |\<in>| ooo_input_op_logic {|0|} os_input"
+    for os' :: "(2, nat \<times> nat + nat set set, nat \<times> nat, (nat, nat) myprod) input_state"
+    using that sorry
+  moreover have "\<exists>op2'. (step Tau)\<^sup>*\<^sup>* (set_spec_op (cUn (cUn S SO) SP) D) op2' \<and> ((~) OO \<U> R OO (\<approx>)) (set_op S D (dataflow_op sg (comp_map (comp_op [Inr (0, 0) \<mapsto> Inr (1, 0)] (case_sum (\<lambda>x. []) (\<lambda>l. map Inr (cbufs l))) (my_ooo_input_op os_input) (loop_op [Inr (2, 0) \<mapsto> Inr (1, 1)] (case_sum (\<lambda>x. []) (\<lambda>l. map Inr (cbufs l))) (comp_map (comp_op [Inr (1, 1) \<mapsto> Inr (2, 0)] (case_sum (\<lambda>x. []) (BENQ (2, 0) (Inr (d, t)) (\<lambda>l. map Inr (cbufs l)))) (my_label_propagation_op (os_label_prop \<lparr>outpu := (outpu os_label_prop)(1 := xs)\<rparr>)) (my_increment_op (os 2))))))))) op2'"
+    if "outpu os_label_prop 1 = (d, t) # xs"
+    for d :: "nat \<times> nat + nat set set"
+      and t :: "(nat, nat) myprod"
+      and xs :: "((nat \<times> nat + nat set set) \<times> (nat, nat) myprod) buf"
+    using that sorry
+  moreover have "\<exists>op2'. (step Tau)\<^sup>*\<^sup>* (set_spec_op (cUn (cUn S SO) SP) D) op2' \<and> ((~) OO \<U> R OO (\<approx>)) (set_op S D (dataflow_op sg (comp_map (comp_op [Inr (0, 0) \<mapsto> Inr (1, 0)] (case_sum (\<lambda>x. []) (\<lambda>l. map Inr (cbufs l))) (my_ooo_input_op os_input) (loop_op [Inr (2, 0) \<mapsto> Inr (1, 1)] (case_sum (\<lambda>x. []) (\<lambda>l. map Inr (cbufs l))) (comp_map (comp_op [Inr (1, 1) \<mapsto> Inr (2, 0)] (case_sum (\<lambda>x. []) (BTL (2, 0) (\<lambda>l. map Inr (cbufs l)))) (my_label_propagation_op os_label_prop) (my_increment_op (consumes (os 2) 0 t d))))))))) op2'"
+    if "cbufs (2, 0) \<noteq> []"
+      and "(d, t) = BHD (2, 0) cbufs"
+    for d :: "nat \<times> nat + nat set set"
+      and t :: "(nat, nat) myprod"
+    using that sorry
+  moreover have "\<exists>op2'. (step Tau)\<^sup>*\<^sup>* (set_spec_op (cUn (cUn S SO) SP) D) op2' \<and> ((~) OO \<U> R OO (\<approx>)) (set_op S D (dataflow_op sg (comp_map (comp_op [Inr (0, 0) \<mapsto> Inr (1, 0)] (case_sum (\<lambda>x. []) (\<lambda>l. map Inr (cbufs l))) (my_ooo_input_op os_input) (loop_op [Inr (2, 0) \<mapsto> Inr (1, 1)] (case_sum (\<lambda>x. []) (\<lambda>l. map Inr (cbufs l))) (comp_map (comp_op [Inr (1, 1) \<mapsto> Inr (2, 0)] (case_sum (\<lambda>x. []) (\<lambda>l. map Inr (cbufs l))) (my_label_propagation_op os') (my_increment_op (os 2))))))))) op2'"
+    if "initia os_label_prop"
+      and "os' |\<in>| label_propagation_op_logic os_label_prop"
+    for os' :: "(nat \<times> nat + nat set set, nat, nat, nat) label_propagation_state"
+    using that sorry
+  moreover have "\<exists>op2'. (step Tau)\<^sup>*\<^sup>* (set_spec_op (cUn (cUn S SO) SP) D) op2' \<and> ((~) OO \<U> R OO (\<approx>)) (set_op S D (dataflow_op sg (comp_map (comp_op [Inr (0, 0) \<mapsto> Inr (1, 0)] (case_sum (\<lambda>x. []) (\<lambda>l. map Inr (cbufs l))) (my_ooo_input_op os_input) (loop_op [Inr (2, 0) \<mapsto> Inr (1, 1)] (case_sum (\<lambda>x. []) (\<lambda>l. map Inr (cbufs l))) (comp_map (comp_op [Inr (1, 1) \<mapsto> Inr (2, 0)] (case_sum (\<lambda>x. []) (\<lambda>l. map Inr (cbufs l))) (my_label_propagation_op os_label_prop) (my_increment_op os')))))))) op2'"
+    if "initia (os 2)"
+      and "os' |\<in>| increment_op_logic 0 0 (MyPair 0 1) (os 2)"
+    for os' :: "(2, nat \<times> nat + nat set set, (nat, nat) myprod) operator_state"
+    using that sorry
+  moreover have "\<exists>op2'. (step Tau)\<^sup>*\<^sup>* (set_spec_op (cUn (cUn S SO) SP) D) op2' \<and> ((~) OO \<U> R OO (\<approx>)) (set_op S D (dataflow_op sg (comp_map (comp_op [Inr (0, 0) \<mapsto> Inr (1, 0)] (case_sum (\<lambda>x. []) (\<lambda>l. map Inr (cbufs l))) (my_ooo_input_op os_input) (loop_op [Inr (2, 0) \<mapsto> Inr (1, 1)] (case_sum (\<lambda>x. []) (BTL (1, 1) (\<lambda>l. map Inr (cbufs l)))) (comp_map (comp_op [Inr (1, 1) \<mapsto> Inr (2, 0)] (case_sum (\<lambda>x. []) (\<lambda>l. map Inr (cbufs l))) (my_label_propagation_op (consumes os_label_prop 1 t d)) (my_increment_op (os 2))))))))) op2'"
+    if "cbufs (1, 1) \<noteq> []"
+      and "(d, t) = BHD (1, 1) cbufs"
+    for d :: "nat \<times> nat + nat set set"
+      and t :: "(nat, nat) myprod"
+    using that sorry
+  moreover have "\<exists>op2'. (step Tau)\<^sup>*\<^sup>* (set_spec_op (cUn (cUn S SO) SP) D) op2' \<and> ((~) OO \<U> R OO (\<approx>)) (set_op S D (dataflow_op sg (comp_map (comp_op [Inr (0, 0) \<mapsto> Inr (1, 0)] (case_sum (\<lambda>x. []) (\<lambda>l. map Inr (cbufs l))) (my_ooo_input_op os_input) (loop_op [Inr (2, 0) \<mapsto> Inr (1, 1)] (case_sum (\<lambda>x. []) (BENQ (1, 1) (Inr (d, t)) (\<lambda>l. map Inr (cbufs l)))) (comp_map (comp_op [Inr (1, 1) \<mapsto> Inr (2, 0)] (case_sum (\<lambda>x. []) (\<lambda>l. map Inr (cbufs l))) (my_label_propagation_op os_label_prop) (my_increment_op (os 2\<lparr>outpu := (outpu (os 2))(0 := xs)\<rparr>))))))))) op2'"
+    if "outpu (os 2) 0 = (d, t) # xs"
+    for d :: "nat \<times> nat + nat set set"
+      and t :: "(nat, nat) myprod"
+      and xs :: "((nat \<times> nat + nat set set) \<times> (nat, nat) myprod) buf"
+    using that sorry
+  moreover have "\<exists>op2'. (step Tau)\<^sup>*\<^sup>* (set_spec_op (cUn (cUn S SO) SP) D) op2' \<and> ((~) OO \<U> R OO (\<approx>)) (set_op S D (dataflow_op (sg\<lparr>upfro := \<lambda>_. True, pt_tr := change_multiplicities (summ sg) (extract_progress 2 (subgraph.nxt sg) st) (pt_tr sg)\<rparr>) (comp_map (comp_op [Inr (0, 0) \<mapsto> Inr (1, 0)] (case_sum (\<lambda>x. []) (\<lambda>l. map Inr (cbufs l))) (my_ooo_input_op os_input) (loop_op [Inr (2, 0) \<mapsto> Inr (1, 1)] (case_sum (\<lambda>x. []) (\<lambda>l. map Inr (cbufs l))) (comp_map (comp_op [Inr (1, 1) \<mapsto> Inr (2, 0)] (case_sum (\<lambda>x. []) (\<lambda>l. map Inr (cbufs l))) (my_label_propagation_op os_label_prop) (my_increment_op os')))))))) op2'"
+    if "(os', st) = obtain_progress (os 2)"
+    for st :: "(2, (nat, nat) myprod) shared_state"
+      and os' :: "(2, nat \<times> nat + nat set set, (nat, nat) myprod) operator_state"
+    using that sorry
+  moreover have "\<exists>op2'. (step Tau)\<^sup>*\<^sup>* (set_spec_op (cUn (cUn S SO) SP) D) op2' \<and> ((~) OO \<U> R OO (\<approx>)) (set_op S D (dataflow_op (sg\<lparr>upfro := \<lambda>_. True, pt_tr := change_multiplicities (summ sg) (extract_progress 1 (subgraph.nxt sg) st) (pt_tr sg)\<rparr>) (comp_map (comp_op [Inr (0, 0) \<mapsto> Inr (1, 0)] (case_sum (\<lambda>x. []) (\<lambda>l. map Inr (cbufs l))) (my_ooo_input_op os_input) (loop_op [Inr (2, 0) \<mapsto> Inr (1, 1)] (case_sum (\<lambda>x. []) (\<lambda>l. map Inr (cbufs l))) (comp_map (comp_op [Inr (1, 1) \<mapsto> Inr (2, 0)] (case_sum (\<lambda>x. []) (\<lambda>l. map Inr (cbufs l))) (my_label_propagation_op os') (my_increment_op (os 2))))))))) op2'"
+    if "(os', st) = obtain_progress os_label_prop"
+    for st :: "(2, (nat, nat) myprod) shared_state"
+      and os' :: "(nat \<times> nat + nat set set, nat, nat, nat) label_propagation_state"
+    using that sorry
+  moreover have "\<exists>op2'. (step Tau)\<^sup>*\<^sup>* (set_spec_op (cUn (cUn S SO) SP) D) op2' \<and> ((~) OO \<U> R OO (\<approx>)) (set_op S D (dataflow_op (sg\<lparr>upfro := \<lambda>_. True, pt_tr := change_multiplicities (summ sg) (extract_progress 0 (subgraph.nxt sg) st) (pt_tr sg)\<rparr>) (comp_map (comp_op [Inr (0, 0) \<mapsto> Inr (1, 0)] (case_sum (\<lambda>x. []) (\<lambda>l. map Inr (cbufs l))) (my_ooo_input_op os') (loop_op [Inr (2, 0) \<mapsto> Inr (1, 1)] (case_sum (\<lambda>x. []) (\<lambda>l. map Inr (cbufs l))) (comp_map (comp_op [Inr (1, 1) \<mapsto> Inr (2, 0)] (case_sum (\<lambda>x. []) (\<lambda>l. map Inr (cbufs l))) (my_label_propagation_op os_label_prop) (my_increment_op (os 2))))))))) op2'"
+    if "(os', st) = obtain_progress os_input"
+    for st :: "(2, (nat, nat) myprod) shared_state"
+      and os' :: "(2, nat \<times> nat + nat set set, nat \<times> nat, (nat, nat) myprod) input_state"
+    using that sorry
+  moreover have "\<exists>op2'. (step Tau)\<^sup>*\<^sup>* (set_spec_op (cUn (cUn S SO) SP) D) op2' \<and> ((~) OO \<U> R OO (\<approx>)) (set_op S D (dataflow_op undefined (comp_map (comp_op [Inr (0, 0) \<mapsto> Inr (1, 0)] (case_sum (\<lambda>x. []) (\<lambda>l. map Inr (cbufs l))) (my_ooo_input_op os_input) (loop_op [Inr (2, 0) \<mapsto> Inr (1, 1)] (case_sum (\<lambda>x. []) (\<lambda>l. map Inr (cbufs l))) (comp_map (comp_op [Inr (1, 1) \<mapsto> Inr (2, 0)] (case_sum (\<lambda>x. []) (\<lambda>l. map Inr (cbufs l))) (my_label_propagation_op (os_label_prop \<lparr>front := frontier \<circ> (\<lambda>p. c_imp (pt_tr undefined) (Loc 1 (Trg p))), initia := True\<rparr>)) (my_increment_op (os 2))))))))) op2'"
+    if "propagate_all (summ sg) (pt_tr sg) = None"
+    using that sorry
+  moreover have "\<exists>op2'. (step Tau)\<^sup>*\<^sup>* (set_spec_op (cUn (cUn S SO) SP) D) op2' \<and> ((~) OO \<U> R OO (\<approx>)) (set_op S D (dataflow_op (sg\<lparr>pt_tr := c, upfro := (upfro sg)(1 := False)\<rparr>) (comp_map (comp_op [Inr (0, 0) \<mapsto> Inr (1, 0)] (case_sum (\<lambda>x. []) (\<lambda>l. map Inr (cbufs l))) (my_ooo_input_op os_input) (loop_op [Inr (2, 0) \<mapsto> Inr (1, 1)] (case_sum (\<lambda>x. []) (\<lambda>l. map Inr (cbufs l))) (comp_map (comp_op [Inr (1, 1) \<mapsto> Inr (2, 0)] (case_sum (\<lambda>x. []) (\<lambda>l. map Inr (cbufs l))) (my_label_propagation_op (os_label_prop \<lparr>front := frontier \<circ> (\<lambda>p. c_imp c (Loc 1 (Trg p))), initia := True\<rparr>)) (my_increment_op (os 2))))))))) op2'"
+    if "propagate_all (summ sg) (pt_tr sg) = Some c"
+    for c :: "((3, 2) location, (nat, nat) myprod) configuration"
+    using that sorry
+  moreover have "\<exists>op2'. (step Tau)\<^sup>*\<^sup>* (set_spec_op (cUn (cUn S SO) SP) D) op2' \<and> ((~) OO \<U> R OO (\<approx>)) (set_op (cinsert ((1, 0), d, t) S) D (dataflow_op sg (comp_map (comp_op [Inr (0, 0) \<mapsto> Inr (1, 0)] (case_sum (\<lambda>x. []) (\<lambda>l. map Inr (cbufs l))) (my_ooo_input_op os_input) (loop_op [Inr (2, 0) \<mapsto> Inr (1, 1)] (case_sum (\<lambda>x. []) (\<lambda>l. map Inr (cbufs l))) (comp_map (comp_op [Inr (1, 1) \<mapsto> Inr (2, 0)] (case_sum (\<lambda>x. []) (\<lambda>l. map Inr (cbufs l))) (my_label_propagation_op (os_label_prop \<lparr>outpu := (outpu os_label_prop)(0 := xs)\<rparr>)) (my_increment_op (os 2))))))))) op2'"
+    if "outpu os_label_prop 0 = (d, t) # xs"
+    for d :: "nat \<times> nat + nat set set"
+      and t :: "(nat, nat) myprod"
+      and xs :: "((nat \<times> nat + nat set set) \<times> (nat, nat) myprod) buf"
+    apply (intro exI conjI)
+    apply (rule rtranclp.rtrancl_refl)
+    apply (intro relcomppI)
+    apply (rule bisim_refl)
+    defer
+    apply (rule wbisim_refl)
+    apply (rule wb_upto_b_base)
+    apply (unfold R_def)
+    apply (rule exI[of _ \<open>cinsert ((1, 0), d, t) S\<close>])
+    apply (rule exI[of _ \<open>cset_from_list (map (\<lambda>x. ((1, 0), x)) xs)\<close>])
+    apply (rule exI[of _ SP])
+    apply (rule exI)
+    apply (rule exI)
+    apply (rule exI[of _ \<open>os(1 := (os 1)\<lparr>outpu := (outpu (os 1))(0 := xs)\<rparr>)\<close>])
+    apply (rule exI)
+    apply (rule exI[of _ \<open>os_label_prop\<lparr>outpu := (outpu os_label_prop)(0 := xs)\<rparr>\<close>])
+    apply (intro exI conjI)
+    apply simp
+    apply (rule arg_cong[where f=\<open>\<lambda>X. set_spec_op (cUn X SP) D\<close>])
+    using SIM1(6,14) that apply (simp add: operator_state.defs(3))
+    apply (simp_all add: SIM1 operator_state.defs(3))
+    using SIM1(3,7) unfolding ty1_check_def apply (simp add: operator_state.defs(3), blast)
+    subgoal
+      using SIM1(6,8) that unfolding ty2_check_def apply -
+      by (simp add: operator_state.defs(3), drule spec[of _ 0], simp)
+    using SIM1(9) unfolding input_ocaps_inv_def apply simp
+    defer
+    apply (subgoal_tac \<open>outputs_at_target (antichain_from_list \<circ>\<circ> raw_summary) (os(1 := (os 1)\<lparr>outpu := (outpu (os 1))(0 := xs)\<rparr>)) (1, 0)
   = outputs_at_target (antichain_from_list \<circ>\<circ> raw_summary) os (1, 0)\<close>)
-      subgoal
-        apply (simp add: BULK_BENQ_def)
-        apply (rule arg_cong[where f=\<open>\<lambda>x. cimage x _\<close>])
-        apply (simp add: fun_eq_iff)
-        apply (rule allI)
-        apply (rule arg_cong[where f=ccs])
-        apply (rule arg_cong[where f=\<open>\<lambda>x. _ \<union> x\<close>])
-        by (simp add: all_edges_def neighbors_def)
-      apply (simp add: outputs_at_target_raw_summary)
-       apply (rule SIM1(15))
-      apply (rule dataplane_tracker_inv_update_outputs_outside)
-         apply (rule SIM1(12))
-      unfolding fun_upd_def apply simp
-      using SIM1(1) apply (simp add: raw_summary_def)
-      sorry
+    subgoal
+      apply (simp add: BULK_BENQ_def)
+      apply (rule arg_cong[where f=\<open>\<lambda>x. cimage x _\<close>])
+      apply (simp add: fun_eq_iff)
+      apply (rule allI)
+      apply (rule arg_cong[where f=ccs])
+      apply (rule arg_cong[where f=\<open>\<lambda>x. _ \<union> x\<close>])
+      by (simp add: all_edges_def neighbors_def)
+    apply (simp add: outputs_at_target_raw_summary)
+    apply (rule SIM1(15))
+    apply (rule dataplane_tracker_inv_update_outputs_outside)
+    apply (rule SIM1(12))
+    unfolding fun_upd_def apply simp
+    using SIM1(1) apply (simp add: raw_summary_def)
+    sorry
 end
-     ultimately show ?thesis
-      (* takes around 70s *)
-      by (use nothing in \<open>((unfold R_def[symmetric], unfold wsim_def my_ooo_input_op_def ooo_input_op_def
+  ultimately show ?thesis
+    (* takes around 70s *)
+    by (use nothing in \<open>((unfold R_def[symmetric], unfold wsim_def my_ooo_input_op_def ooo_input_op_def
           my_label_propagation_op_def label_propagation_op_def my_increment_op_def increment_op_def,
           intro allI impI, elim step_dataflow_op_elim step_set_op_elim step_map_op_elim step_comp_op_elim
           step_builder_op_elim conjE; simp only: IO.simps; hypsubst_thin?; (elim step_map_op_elim
@@ -514,7 +620,7 @@ end
         clarsimp split: if_splits option.splits dest!: num2_neq simp flip: my_ooo_input_op_def ooo_input_op_def
           my_label_propagation_op_def label_propagation_op_def my_increment_op_def increment_op_def; hypsubst_thin?),
         use method_facts in simp_all\<close>)
-  qed
+qed
 next
   case SIM2
   then show ?case sorry
